FInish invariant proof

theories/examples/coupon.v
@@ -1,7 +1,7 @@
 (* A case study of coupon collection *)
 From clutch Require Export clutch.
 From clutch.lib Require Export map.
-From stdpp Require Export fin_maps. 
+From stdpp Require Export fin_maps fin_sets finite. 
 
 
 Set Default Proof Using "Type*".
@@ -58,20 +58,20 @@ Section proofs.
   Definition couponN := nroot.@"coupon".
   
 
-  Definition map_set_relate start n (m: gmap nat val) (s:gset nat)  :=
-    forall elem, elem ∈ s <-> is_Some (m !! elem) /\ start <= elem < n.
+  Definition map_set_relate (m: gmap nat val) (s:gset nat)  :=
+    forall elem, elem ∈ s <-> is_Some (m !! elem).
 
   (* This is an invariant in the sense that it holds true for every recursive call, 
      but we do not technically allocate it as an invariant in the RA sense. 
    *)
   Definition coupon_collection_inv n lm (k:Z) (cnt cnt' : loc): iProp Σ :=
     (∃(cntv : nat) s m,
-        map_list lm m ∗ ⌜map_set_relate 0 n m s⌝ ∗ cnt' ↦ₛ #cntv ∗ cnt ↦ #cntv ∗ ⌜Z.of_nat (size s) = k⌝ )%I.
+        map_list lm m ∗ ⌜map_set_relate m s⌝ ∗ cnt' ↦ₛ #cntv ∗ cnt ↦ #cntv ∗ ⌜Z.of_nat (size s) = k⌝ ∗⌜s∩set_seq 0 n = s⌝ )%I.
 
   
   Lemma wp_cnt_map_helper E lm m n s start:
     start <= n ->
-    map_set_relate start n m s ->
+    map_set_relate m s ->
     {{{ map_list lm m ∗ ⌜s∩set_seq 0 n = s⌝}}}
       cnt_map_helper #lm #start #n @ E
       {{{v, RET #v; map_list lm m ∗ ⌜v = size (s ∩ (set_seq start (n-start)))⌝
@@ -79,72 +79,153 @@ Section proofs.
       }}}.
   Proof. 
     iIntros (H Hms Φ) "[(%&%&Hlm&%&Ha) %] HΦ".
-    (* wp_pure. *)
-    (* iRevert (H H0 Hms Φ) "HΦ". *)
-    (* iLöb as "IH" forall (start lv vs). *)
-    (* iIntros "%H %H0 %Hms %Φ HΦ". *)
-    (* wp_pures. *)
-    (* case_bool_decide. *)
-    (* - wp_pures. iModIntro. replace 0%Z with (Z.of_nat 0) by lia. *)
-    (*   iApply ("HΦ" with "[Hlm Ha]"). *)
-    (*   rewrite /map_list. *)
-    (*   iSplitL. *)
-    (*   + iExists _, _. iFrame. by iPureIntro. *)
-    (*   + subst. iPureIntro. rewrite /map_set_relate in Hms. *)
-    (*     inversion H1. rewrite Nat2Z.inj_iff in H2. subst => /=. *)
-    (*     assert (set_seq n (n-n) = (∅ : gset nat)). *)
-    (*     { rewrite elem_of_equiv_empty_L. intros. intro. rewrite elem_of_set_seq in H0. *)
-    (*       destruct H0. lia. *)
-    (*     } rewrite H0. *)
-    (*     assert (s∩∅ = ∅). *)
-    (*     { rewrite elem_of_equiv_empty_L. intros. intro. *)
-    (*       rewrite elem_of_intersection in H2. *)
-    (*       destruct H2. *)
-    (*       by rewrite elem_of_empty in H3. *)
-    (*     } *)
-    (*     rewrite H2. done. *)
-    (* - wp_pures. wp_bind (get _ _). *)
-    (*   wp_apply (wp_get with "[Hlm Ha]"). *)
-    (*   { iExists _, _. iFrame. by iPureIntro. } *)
-    (*   iIntros (b) "[ (%&%&Hlm&%&Ha) %Hres]". *)
-    (*   subst. *)
-    (*   destruct (list_to_map vs !! start) eqn:Hd. *)
-    (*   + do 3 wp_pure. *)
-    (*     replace (Z.of_nat start + 1)%Z with (Z.of_nat (S start)) by lia. *)
-    (*     wp_bind (App _ _)%E. *)
-    (*     wp_apply (wp_mono with "[Hlm Ha]"); last first. *)
-    (*     { wp_apply ("IH" with "[$Hlm][$Ha]"). *)
-    (*       - iPureIntro. assert (start ≠ n). *)
-    (*         { intro. subst. done. } *)
-    (*         assert (start < n) by lia. *)
-    (*         lia. *)
-    (*       - done. *)
-    (*       - admit. *)
-    (*       - admit. *)
-    (*     } *)
-    (*     intros. *)
-        
-    (*     admit. *)
-    (*   + do 3 wp_pure. *)
-    (*     replace (Z.of_nat start + 1)%Z with (Z.of_nat (S start)) by lia. *)
-    (*     iApply ("IH" with "[$Hlm][$Ha]"). *)
-    (*     -- iPureIntro. destruct H; try done. lia. *)
-    (*     -- by iPureIntro. *)
-    (*     -- iPureIntro. intro. split; intros. *)
-    (*        ++ apply Hms in H0. destruct H0. split; try done. *)
-    (*           destruct H3. split; try done. *)
-    (*           destruct H3; try lia. rewrite Hd in H0. inversion H0. done. *)
-    (*        ++ rewrite Hms. destruct H0. split; try done. *)
-    (*           destruct H3; split; try done. *)
-    (*           lia. *)
-    (*     -- admit.       *)
-  Admitted.
+    wp_pure.
+    iRevert (H H0 Hms Φ) "HΦ".
+    iLöb as "IH" forall (start lv vs).
+    iIntros "%H %H0 %Hms %Φ HΦ".
+    wp_pures.
+    case_bool_decide.
+    - wp_pures. iModIntro. replace 0%Z with (Z.of_nat 0) by lia.
+      iApply ("HΦ" with "[Hlm Ha]").
+      rewrite /map_list.
+      iSplitL.
+      + iExists _, _. iFrame. by iPureIntro.
+      + subst. iPureIntro. rewrite /map_set_relate in Hms.
+        inversion H2. rewrite Nat2Z.inj_iff in H3. subst => /=.
+        assert (set_seq n (n-n) = (∅ : gset nat)).
+        { rewrite elem_of_equiv_empty_L. intros. intro. rewrite elem_of_set_seq in H0.
+          destruct H0. lia.
+        } rewrite H0.
+        assert (s∩∅ = ∅).
+        { rewrite elem_of_equiv_empty_L. intros. intro.
+          replace (s ∩ ∅) with (∅:gset nat) in H3.
+          2: { symmetry. rewrite <- (disjoint_intersection_L). apply disjoint_empty_r. } 
+          by rewrite elem_of_empty in H3.
+        }
+        split.
+        -- rewrite H3. done.
+        -- done. 
+    - wp_pures. wp_bind (get _ _).
+      wp_apply (wp_get with "[Hlm Ha]").
+      { iExists _, _. iFrame. by iPureIntro. }
+      iIntros (b) "[ (%&%&Hlm&%&Ha) %Hres]".
+      subst.
+      destruct (list_to_map vs !! start) eqn:Hd.
+      + do 3 wp_pure.
+        replace (Z.of_nat start + 1)%Z with (Z.of_nat (S start)) by lia.
+        wp_bind (App _ _)%E.
+        wp_apply (wp_mono with "[Hlm Ha HΦ]"); last first.
+        { wp_apply ("IH" with "[$Hlm][$Ha][][][][HΦ]").
+          - iPureIntro. assert (start ≠ n).
+            { intro. subst. done. }
+            assert (start < n) by lia.
+            lia.
+          - done.
+          - iPureIntro. split.
+            + intros H'. by apply Hms in H'.
+            + intros.
+              by rewrite Hms. 
+          - iIntros (?) "(?&%&%)".
+            instantiate (1 :=
+                           (λ v': val, ∃ v0 : nat, (⌜#v0 = v'⌝∗ map_list lm (list_to_map vs) ∗ ⌜v0 =(size (s ∩ set_seq (S start) (n - S start)))⌝ ∗ ⌜s ∩ set_seq 0 n = s⌝) ∗
+                           (∀ v1 : nat,
+           map_list lm (list_to_map vs) ∗ ⌜v1 = size (s ∩ set_seq start (n - start))⌝ ∗
+           ⌜s ∩ set_seq 0 n = s⌝ -∗ Φ #v1))%I).
+            simpl. iFrame.
+            iExists _.
+            iSplitR; [done|].
+            iPureIntro. split; try done. 
+        }
+        intros. simpl.
+        iIntros "[%((<-&Hml&%&%)&HΦ)]".
+        wp_pures.
+        iModIntro.
+        replace (Z.of_nat v1 + 1)%Z with (Z.of_nat (S v1)) by lia.
+        iApply ("HΦ" with "[Hml]"); iFrame.
+        iPureIntro.
+        split; try done.
+        rewrite H0.
+        assert (start ∈ s).
+        { rewrite Hms. rewrite Hd. done. }
+        replace (_∩ set_seq start _) with ({[start]}∪(s ∩ set_seq (S start) (n - S start))).
+        -- rewrite size_union.
+           { rewrite size_singleton. lia. }
+           rewrite disjoint_singleton_l.
+           rewrite elem_of_intersection.
+           intros [??].
+           rewrite elem_of_set_seq in H7. lia.
+        -- rewrite set_eq. intros. split; intros K.
+           --- rewrite elem_of_union in K. destruct K as [K|K].
+               +++ rewrite elem_of_singleton in K. subst.
+                   rewrite elem_of_intersection. split; try done.
+                   rewrite elem_of_set_seq. split; try lia.
+                   assert (start ≠ n).
+                   { intro; subst; done. }
+                   lia.
+               +++ rewrite elem_of_intersection in K.
+                   destruct K as [K K'].
+                   rewrite elem_of_intersection. split; try done.
+                   rewrite elem_of_set_seq. rewrite elem_of_set_seq in K'.
+                   destruct K'.
+                   split; try lia.
+           --- rewrite elem_of_intersection in K. destruct K as [K K'].
+               rewrite elem_of_union. 
+               rewrite elem_of_intersection.
+               rewrite elem_of_set_seq. rewrite elem_of_set_seq in K'.
+               destruct K' as [K' K''].
+               destruct (decide (x=start)).
+               +++ left. subst. by apply elem_of_singleton.
+               +++ right.
+                   split; try done.
+                   split; try lia.
+      + do 3 wp_pure.
+        replace (Z.of_nat start + 1)%Z with (Z.of_nat (S start)) by lia.
+        iApply ("IH" with "[$Hlm][$Ha]").
+        -- iPureIntro. destruct H; try done. lia.
+        -- by iPureIntro.
+        -- iPureIntro. intro. split; intros.
+           ++ by apply Hms in H0.  
+           ++ rewrite Hms. destruct H0. rewrite H0. done. 
+        -- iIntros (?) "(?&%&%)".
+           iApply "HΦ".
+           iFrame.
+           iPureIntro; split; try done.
+           rewrite H0.
+           assert (start ∉ s).
+           { intro. rewrite Hms in H5. rewrite Hd in H5. inversion H5. done. }
+           f_equal.
+           rewrite set_eq. intros. split; intros.
+           ++ rewrite elem_of_intersection in H6. destruct H6 as [H6 H6'].
+              rewrite elem_of_intersection; split; try done.
+              rewrite elem_of_set_seq in H6'. destruct H6'. rewrite elem_of_set_seq.
+              split; try lia.
+           ++ rewrite elem_of_intersection. rewrite elem_of_intersection in H6. 
+              destruct H6. split; try done.
+              rewrite elem_of_set_seq in H7. rewrite elem_of_set_seq. split; try lia.
+              assert (x≠start).
+              { intro. subst. done. }
+              lia.
+Qed.              
 
   
 
   Lemma coupon_bijection n m s (k:Z):
-    map_set_relate 0 n m s -> Z.of_nat (size s) = k ->
+    n>0 -> map_set_relate m s -> Z.of_nat (size s) = k -> s∩set_seq 0 n = s ->
     ∃ f: (fin (S(n-1))) -> fin (S (n-1)), Bij f /\ forall x, f x < Z.to_nat k <-> is_Some (m!! fin_to_nat x).
+  Proof.
+    intros H0 H1 H2 H3.
+    apply subseteq_intersection_2_L in H3.
+    rewrite elem_of_subseteq in H3.
+    rewrite /map_set_relate in H1.
+    assert (∃ f : fin (S (n - 1)) → fin (S (n - 1)),
+               Bij f ∧ (∀ x : fin (S (n - 1)), f x < Z.to_nat k ↔ fin_to_nat x ∈ s)); last first.
+    { destruct H as [f[??]]. exists f. split; try done. intros; split; intros.
+      - rewrite <- H1. rewrite <- H4. done.
+      - rewrite H4.  rewrite H1. done.
+    }
+    clear m H1.
+    replace (S (n-1)) with n by lia.
+    
     Admitted. 
 
   Lemma coupon_collection_refines_spec_helper n lm (k:Z) cnt cnt':
@@ -159,7 +240,7 @@ Section proofs.
     iRevert "Inv".
     iLöb as "IH" forall (k).
     iIntros "Inv".
-    iDestruct "Inv" as (???) "(Hml&%Hms&Hc'&Hc&%)".
+    iDestruct "Inv" as (???) "(Hml&%Hms&Hc'&Hc&%&%)".
     do 9 rel_pure_l. 
     rewrite -!/cnt_map_helper.
     rel_pures_r.
@@ -179,11 +260,14 @@ Section proofs.
           intro.
           intros.
           rewrite elem_of_set_seq.
-          rewrite Hms in H0. lia.  
+          split; try lia.
+          simpl.
+          rewrite <-H1 in H0.
+          rewrite elem_of_intersection in H0. destruct H0. rewrite elem_of_set_seq in H3. lia.
       }
-      iModIntro. iIntros (?) "[?[%%]]". rewrite H1. rewrite H0.
+      iModIntro. iIntros (?) "[?[%%]]". rewrite H2. rewrite H0.
       rel_pures_l. case_bool_decide; last first.
-      { exfalso. apply H3. f_equal. replace (n-0) with n by lia. rewrite H2.  done. }
+      { exfalso. apply H4. f_equal. replace (n-0) with n by lia. rewrite H3.  done. }
       rel_pures_l.
       rel_load_l.
       rel_values.
@@ -204,20 +288,23 @@ Section proofs.
           intro.
           intros.
           rewrite elem_of_set_seq.
-          rewrite Hms in H2. lia.  
+          split; try lia.
+          simpl.
+          rewrite <- H1 in H3. rewrite elem_of_intersection in H3. destruct H3.
+          rewrite elem_of_set_seq in H4. destruct H4. lia. 
       }
-      iModIntro. iIntros (?) "[Hml [%%]]". rewrite H2.
+      iModIntro. iIntros (?) "[Hml [%%]]". rewrite H3.
       rel_pures_l.
       case_bool_decide.
-      { replace (n-0) with n in H4 by lia. rewrite H3 in H4.
-        rewrite H0 in H4. done. }
+      { replace (n-0) with n in H5 by lia. rewrite H4 in H5.
+        rewrite H0 in H5. done. }
       rel_pures_l.
       rel_load_l.
       rel_pures_l.
       rel_store_l.
       rel_pures_l.
       clear H1 H2 H3. 
-      destruct (coupon_bijection _ _ _ _ Hms H0) as [f[]].
+      destruct (coupon_bijection _ _ _ _ H  Hms H0 H4) as [f[]].
       rel_apply (refines_couple_UU _ f).
       { by replace (Z.to_nat (Z.of_nat n - 1)) with (n-1) by lia. }
       iModIntro. iIntros (r).
@@ -233,30 +320,31 @@ Section proofs.
         iExists _, ({[fin_to_nat r]} ∪ s), _.
         replace (Z.of_nat cntv + 1)%Z with (Z.of_nat (S cntv)) by lia.
         iFrame.
-        clear H4. 
         iSplit; iPureIntro. 
         -- intros. split; intros; try split.
            ++ rewrite lookup_insert_is_Some'.
-              apply elem_of_union in H4 as [H4|H4].
-              --- rewrite elem_of_singleton in H4. subst.
+              apply elem_of_union in H6 as [H6|H6].
+              --- rewrite elem_of_singleton in H6. subst.
                   by left.
-              --- right. apply Hms in H4. by destruct H4.
-           ++ split; try lia.
-              apply elem_of_union in H4 as [H4|H4].
-              --- rewrite elem_of_singleton in H4. subst.
-                  replace n with (S (n-1)) by lia.
-                  apply fin_to_nat_lt.
-              --- apply Hms in H4. by destruct H4 as [?[]].
-           ++ destruct H4.
-              rewrite lookup_insert_is_Some' in H4.
+              --- right. apply Hms in H6. by destruct H6.
+           ++ rewrite lookup_insert_is_Some' in H6.
               apply elem_of_union.
-              destruct H4.
+              destruct H6.
               --- left. by apply elem_of_singleton.
-              --- right. rewrite Hms. by split.
+              --- right. rewrite Hms. done. 
         -- rewrite size_union.
-           ++ rewrite size_singleton. lia.
-           ++ rewrite disjoint_singleton_l. intro. apply Hms in H4 as [??].
-              rewrite <-H2 in H4. lia. 
+           ++ rewrite size_singleton. split; first lia.
+              apply subseteq_intersection_1_L.
+              rewrite union_subseteq.
+              split.
+              --- rewrite singleton_subseteq_l.
+                  rewrite elem_of_set_seq.
+                  split; simpl; try lia.
+                  pose proof (fin_to_nat_lt r).
+                  lia.
+              --- by apply subseteq_intersection_2_L in H4. 
+           ++ rewrite disjoint_singleton_l. intro. rewrite Hms in H6.
+              rewrite <- H2 in H6. apply Zgt_not_le in H3; lia.
       + (* old coupon *)
         do 2 rel_pure_l.
         rel_pure_r.
@@ -264,20 +352,18 @@ Section proofs.
         iExists _, s, _.
         replace (Z.of_nat cntv + 1)%Z with (Z.of_nat (S cntv)) by lia.
         iFrame.
-        clear H4. 
         iSplit; iPureIntro.        
         -- split; intros; try split.
-           ++ apply Hms in H4 as [].
+           ++ apply Hms in H6 as [].
               rewrite lookup_insert_is_Some'.
               by right.
-           ++ by apply Hms in H4 as [].
-           ++ rewrite Hms. destruct H4; split; try done.
-              rewrite lookup_insert_is_Some' in H4.
-              destruct H4.
+           ++ rewrite Hms. 
+              rewrite lookup_insert_is_Some' in H6.
+              destruct H6.
               --- subst. rewrite -H2.
                   lia.
               --- done.
-        -- done.
+        -- split; try done.
  Qed. 
     
   Lemma coupon_collection_refines_spec n:
@@ -300,9 +386,11 @@ Section proofs.
     iExists _. iFrame.
     iSplit.
     - iPureIntro. intros. split; intros; [by rewrite elem_of_empty in H0|]. 
-      destruct H0 as [H' ?]. rewrite lookup_empty in H'. destruct H' as [H'?].
-      inversion H1. 
-    - iPureIntro. done. 
+      destruct H0 as [? H']. rewrite lookup_empty in H'.
+      inversion H'. 
+    - iPureIntro. split; try done.
+      apply disjoint_intersection_L.
+      done.
   Qed. 
 
   
